coq: Add a mux-elimination pass to simplify ‘Mux(s, γ, γ)’ into ‘γ’
We can't always afford to check for complete circuit equality, so we allow an
incomplete Boolean decider and wire that to OCaml's physical equality (==).

ocaml/cuttlebone/cuttlebone.ml
@@ -271,11 +271,17 @@ module Compilation = struct
     Extr.type_rule Util.string_eq_dec _R _Sigma pos (Extr.desugar_action pos ast)
     |> result_of_type_result
 
+  let opt _R _Sigma =
+    let open Extr in
+    let eqb _ c1 c2 = c1 == c2 in
+    let cR, cSigma = cR_of_R _R, cSigma_of_Sigma _Sigma in
+    lco_opt_compose cR cSigma (opt_constprop cR cSigma) (opt_muxelim cR cSigma eqb)
+
   let compile (cu: 'f compile_unit) : (reg_signature -> compiled_circuit) =
     let finiteType = finiteType_of_register_list cu.c_registers in
     let rules r = List.assoc r cu.c_rules |> snd in
     let rEnv = Extr.contextEnv finiteType in
-    let env = Extr.compile_scheduler _R _Sigma finiteType rules cu.c_scheduler in
+    let env = Extr.compile_scheduler _R _Sigma finiteType (opt _R _Sigma) rules cu.c_scheduler in
     (fun r -> Extr.getenv rEnv env r)
 end
 
@@ -470,7 +476,7 @@ module Graphs = struct
     let di_regs =
       kp.koika_reg_finite.finite_elements in
     let di_circuits =
-      let cp = Extr.compile_koika_package kp in
+      let cp = Extr.compile_koika_package kp (Compilation.opt kp.koika_reg_types kp.koika_ext_fn_types) in
       fun r -> Extr.getenv cp.cp_reg_Env cp.cp_circuits r in
     let di_fn_sigs f =
       let fn_name = Util.string_of_coq_string (vp.vp_ext_fn_names f) in
